src/dafny_go/bytes/bytes_test.go
@@ -44,3 +44,19 @@ func TestCopyTo(t *testing.T) {
 
 	assert.Equal(t, []byte{0, 4}, bs2.Data)
 }
+
+func TestSplit(t *testing.T) {
+	bs := NewBytes(3)
+	bs.Data[1] = 1
+	bs2 := bs.Split(1)
+
+	assert.Equal(t, uint64(1), bs.Len())
+	assert.Equal(t, uint64(2), bs2.Len())
+
+	assert.Equal(t, []byte{0}, bs.Data)
+	assert.Equal(t, []byte{1, 0}, bs2.Data)
+
+	bs.Append(2)
+	assert.Equal(t, byte(2), bs.Get(1), "we just wrote that")
+	assert.Equal(t, byte(1), bs2.Get(0), "Split did not create independent slice")
+}
