src/Dafny/util/min_max.dfy
@@ -1,0 +1,11 @@
+module MinMax {
+  function method min(x: int, y: int): int
+  {
+    if x < y then x else y
+  }
+
+  function method max(x: int, y: int): int
+  {
+    if x < y then y else x
+  }
+}
